src/ocaml-output/FStar_TypeChecker_Core.ml
@@ -1,7 +1,31 @@
 open Prims
+type env =
+  {
+  tcenv: FStar_TypeChecker_Env.env ;
+  allow_universe_instantiation: Prims.bool }
+let (__proj__Mkenv__item__tcenv : env -> FStar_TypeChecker_Env.env) =
+  fun projectee ->
+    match projectee with | { tcenv; allow_universe_instantiation;_} -> tcenv
+let (__proj__Mkenv__item__allow_universe_instantiation : env -> Prims.bool) =
+  fun projectee ->
+    match projectee with
+    | { tcenv; allow_universe_instantiation;_} ->
+        allow_universe_instantiation
+let (push_binders : env -> FStar_Syntax_Syntax.binders -> env) =
+  fun g ->
+    fun bs ->
+      let uu___ = FStar_TypeChecker_Env.push_binders g.tcenv bs in
+      {
+        tcenv = uu___;
+        allow_universe_instantiation = (g.allow_universe_instantiation)
+      }
 type precondition = FStar_Syntax_Syntax.typ FStar_Pervasives_Native.option
 type 'a success = ('a * precondition)
-type 'a result = ('a success, Prims.string) FStar_Pervasives.either
+type context =
+  (Prims.string * FStar_Syntax_Syntax.term FStar_Pervasives_Native.option)
+    Prims.list
+type error = (context * Prims.string)
+type 'a result = context -> ('a success, error) FStar_Pervasives.either
 type hash_entry =
   {
   he_term: FStar_Syntax_Syntax.term ;
@@ -23,8 +47,7 @@ type tc_table = (FStar_Syntax_Syntax.term, hash_entry) FStar_Hash.hashtable
 let (table : tc_table) = FStar_Hash.create FStar_Syntax_Hash.equal_term
 let (clear_memo_table : unit -> unit) = fun uu___ -> FStar_Hash.clear table
 let (insert :
-  FStar_TypeChecker_Env.env ->
-    FStar_Syntax_Syntax.term -> FStar_Syntax_Syntax.typ success -> unit)
+  env -> FStar_Syntax_Syntax.term -> FStar_Syntax_Syntax.typ success -> unit)
   =
   fun g ->
     fun e ->
@@ -32,12 +55,13 @@ let (insert :
         let entry =
           {
             he_term = e;
-            he_gamma = (g.FStar_TypeChecker_Env.gamma);
+            he_gamma = ((g.tcenv).FStar_TypeChecker_Env.gamma);
             he_res = res
           } in
         FStar_Hash.insert (e, FStar_Syntax_Hash.hash_term) entry table
 let return : 'a . 'a -> 'a result =
-  fun x -> FStar_Pervasives.Inl (x, FStar_Pervasives_Native.None)
+  fun x ->
+    fun uu___ -> FStar_Pervasives.Inl (x, FStar_Pervasives_Native.None)
 let (and_pre :
   precondition ->
     precondition ->
@@ -60,32 +84,44 @@ let (and_pre :
 let bind : 'a 'b . 'a result -> ('a -> 'b result) -> 'b result =
   fun x ->
     fun y ->
-      match x with
-      | FStar_Pervasives.Inl (x1, g1) ->
-          let uu___ = y x1 in
-          (match uu___ with
-           | FStar_Pervasives.Inl (y1, g2) ->
-               let uu___1 = let uu___2 = and_pre g1 g2 in (y1, uu___2) in
-               FStar_Pervasives.Inl uu___1
-           | err -> err)
-      | FStar_Pervasives.Inr err -> FStar_Pervasives.Inr err
+      fun ctx0 ->
+        let uu___ = x ctx0 in
+        match uu___ with
+        | FStar_Pervasives.Inl (x1, g1) ->
+            let uu___1 = let uu___2 = y x1 in uu___2 ctx0 in
+            (match uu___1 with
+             | FStar_Pervasives.Inl (y1, g2) ->
+                 let uu___2 = let uu___3 = and_pre g1 g2 in (y1, uu___3) in
+                 FStar_Pervasives.Inl uu___2
+             | err -> err)
+        | FStar_Pervasives.Inr err -> FStar_Pervasives.Inr err
 let fail : 'a . Prims.string -> 'a result =
-  fun msg -> FStar_Pervasives.Inr msg
+  fun msg -> fun ctx -> FStar_Pervasives.Inr (ctx, msg)
 let handle_with : 'a . 'a result -> (unit -> 'a result) -> 'a result =
   fun x ->
-    fun h -> match x with | FStar_Pervasives.Inr uu___ -> h () | res -> res
+    fun h ->
+      fun ctx ->
+        let uu___ = x ctx in
+        match uu___ with
+        | FStar_Pervasives.Inr uu___1 -> let uu___2 = h () in uu___2 ctx
+        | res -> res
+let with_context :
+  'a .
+    Prims.string ->
+      FStar_Syntax_Syntax.term FStar_Pervasives_Native.option ->
+        (unit -> 'a result) -> 'a result
+  =
+  fun msg ->
+    fun t -> fun x -> fun ctx -> let uu___ = x () in uu___ ((msg, t) :: ctx)
 let (mk_type :
   FStar_Syntax_Syntax.universe ->
     FStar_Syntax_Syntax.term' FStar_Syntax_Syntax.syntax)
   =
   fun u ->
-    FStar_Syntax_Syntax.mk
-      (FStar_Syntax_Syntax.Tm_type (FStar_Syntax_Syntax.U_succ u))
+    FStar_Syntax_Syntax.mk (FStar_Syntax_Syntax.Tm_type u)
       FStar_Compiler_Range.dummyRange
 let (is_type :
-  FStar_TypeChecker_Env.env ->
-    FStar_Syntax_Syntax.term -> FStar_Syntax_Syntax.universe result)
-  =
+  env -> FStar_Syntax_Syntax.term -> FStar_Syntax_Syntax.universe result) =
   fun g ->
     fun t ->
       let aux t1 =
@@ -95,15 +131,18 @@ let (is_type :
         match uu___ with
         | FStar_Syntax_Syntax.Tm_type u -> return u
         | uu___1 -> fail "Expected a type" in
-      let uu___ = aux t in
-      handle_with uu___
-        (fun uu___1 ->
-           let uu___2 =
-             let uu___3 = FStar_TypeChecker_Normalize.unfold_whnf g t in
-             FStar_Syntax_Util.unrefine uu___3 in
-           aux uu___2)
+      with_context "is_type" FStar_Pervasives_Native.None
+        (fun uu___ ->
+           let uu___1 = aux t in
+           handle_with uu___1
+             (fun uu___2 ->
+                let uu___3 =
+                  let uu___4 =
+                    FStar_TypeChecker_Normalize.unfold_whnf g.tcenv t in
+                  FStar_Syntax_Util.unrefine uu___4 in
+                aux uu___3))
 let (is_tot_arrow :
-  FStar_TypeChecker_Env.env ->
+  env ->
     FStar_Syntax_Syntax.term ->
       (FStar_Syntax_Syntax.binder * FStar_Syntax_Syntax.typ) result)
   =
@@ -130,30 +169,33 @@ let (is_tot_arrow :
             let uu___1 = FStar_Syntax_Subst.open_term [x] t2 in
             (match uu___1 with | (x1::[], t3) -> return (x1, t3))
         | uu___1 -> fail "Expected an arrow" in
-      let uu___ = aux t in
-      handle_with uu___
-        (fun uu___1 ->
-           let uu___2 = FStar_TypeChecker_Normalize.unfold_whnf g t in
-           aux uu___2)
+      with_context "is_tot_arrow" FStar_Pervasives_Native.None
+        (fun uu___ ->
+           let uu___1 = aux t in
+           handle_with uu___1
+             (fun uu___2 ->
+                let uu___3 =
+                  FStar_TypeChecker_Normalize.unfold_whnf g.tcenv t in
+                aux uu___3))
 let (check_arg_qual :
   FStar_Syntax_Syntax.aqual -> FStar_Syntax_Syntax.bqual -> unit result) =
   fun a ->
     fun b ->
-      match (b, a) with
-      | (FStar_Pervasives_Native.None, FStar_Pervasives_Native.None) ->
-          return ()
-      | (FStar_Pervasives_Native.Some (FStar_Syntax_Syntax.Implicit uu___),
-         FStar_Pervasives_Native.Some
-         { FStar_Syntax_Syntax.aqual_implicit = true;
-           FStar_Syntax_Syntax.aqual_attributes = uu___1;_})
-          -> return ()
-      | (FStar_Pervasives_Native.Some uu___, FStar_Pervasives_Native.None) ->
-          return ()
-      | (FStar_Pervasives_Native.Some uu___, FStar_Pervasives_Native.Some
-         { FStar_Syntax_Syntax.aqual_implicit = false;
-           FStar_Syntax_Syntax.aqual_attributes = uu___1;_})
-          -> return ()
-      | uu___ -> fail "Arg qualfier mismatch"
+      match b with
+      | FStar_Pervasives_Native.Some (FStar_Syntax_Syntax.Implicit uu___) ->
+          (match a with
+           | FStar_Pervasives_Native.Some
+               { FStar_Syntax_Syntax.aqual_implicit = true;
+                 FStar_Syntax_Syntax.aqual_attributes = uu___1;_}
+               -> return ()
+           | uu___1 -> fail "missing arg qualifier implicit")
+      | uu___ ->
+          (match a with
+           | FStar_Pervasives_Native.Some
+               { FStar_Syntax_Syntax.aqual_implicit = true;
+                 FStar_Syntax_Syntax.aqual_attributes = uu___1;_}
+               -> fail "extra arg qualifier implicit"
+           | uu___1 -> return ())
 let (check_bqual :
   FStar_Syntax_Syntax.bqual -> FStar_Syntax_Syntax.bqual -> unit result) =
   fun b0 ->
@@ -216,11 +258,13 @@ let with_binders :
   fun xs ->
     fun us ->
       fun f ->
-        match f with
-        | FStar_Pervasives.Inl (t, g) ->
-            let uu___ = let uu___1 = close_guard xs us g in (t, uu___1) in
-            FStar_Pervasives.Inl uu___
-        | err -> err
+        fun ctx ->
+          let uu___ = f ctx in
+          match uu___ with
+          | FStar_Pervasives.Inl (t, g) ->
+              let uu___1 = let uu___2 = close_guard xs us g in (t, uu___2) in
+              FStar_Pervasives.Inl uu___1
+          | err -> err
 let with_definition :
   'a .
     FStar_Syntax_Syntax.binder ->
@@ -231,15 +275,18 @@ let with_definition :
     fun u ->
       fun t ->
         fun f ->
-          match f with
-          | FStar_Pervasives.Inl (a1, g) ->
-              let uu___ =
-                let uu___1 = close_guard_with_definition x u t g in
-                (a1, uu___1) in
-              FStar_Pervasives.Inl uu___
-          | err -> err
+          fun ctx ->
+            let uu___ = f ctx in
+            match uu___ with
+            | FStar_Pervasives.Inl (a1, g) ->
+                let uu___1 =
+                  let uu___2 = close_guard_with_definition x u t g in
+                  (a1, uu___2) in
+                FStar_Pervasives.Inl uu___1
+            | err -> err
 let (guard : FStar_Syntax_Syntax.typ -> unit result) =
-  fun t -> FStar_Pervasives.Inl ((), (FStar_Pervasives_Native.Some t))
+  fun t ->
+    fun uu___ -> FStar_Pervasives.Inl ((), (FStar_Pervasives_Native.Some t))
 let (abs :
   FStar_Syntax_Syntax.typ ->
     (FStar_Syntax_Syntax.binder -> FStar_Syntax_Syntax.term) ->
@@ -269,28 +316,33 @@ let (strengthen_subtyping_guard :
 let weaken :
   'a .
     FStar_Syntax_Syntax.term ->
-      'a result -> ('a success, Prims.string) FStar_Pervasives.either
+      'a result -> context -> ('a success, error) FStar_Pervasives.either
   =
   fun p ->
     fun g ->
-      match g with
-      | FStar_Pervasives.Inl (x, q) ->
-          let uu___ = let uu___1 = weaken_subtyping_guard p q in (x, uu___1) in
-          FStar_Pervasives.Inl uu___
-      | err -> err
+      fun ctx ->
+        let uu___ = g ctx in
+        match uu___ with
+        | FStar_Pervasives.Inl (x, q) ->
+            let uu___1 =
+              let uu___2 = weaken_subtyping_guard p q in (x, uu___2) in
+            FStar_Pervasives.Inl uu___1
+        | err -> err
 let strengthen :
   'a .
     FStar_Syntax_Syntax.term ->
-      'a result -> ('a success, Prims.string) FStar_Pervasives.either
+      'a result -> context -> ('a success, error) FStar_Pervasives.either
   =
   fun p ->
     fun g ->
-      match g with
-      | FStar_Pervasives.Inl (x, q) ->
-          let uu___ =
-            let uu___1 = strengthen_subtyping_guard p q in (x, uu___1) in
-          FStar_Pervasives.Inl uu___
-      | err -> err
+      fun ctx ->
+        let uu___ = g ctx in
+        match uu___ with
+        | FStar_Pervasives.Inl (x, q) ->
+            let uu___1 =
+              let uu___2 = strengthen_subtyping_guard p q in (x, uu___2) in
+            FStar_Pervasives.Inl uu___1
+        | err -> err
 let (equatable :
   FStar_Syntax_Syntax.term -> FStar_Syntax_Syntax.term -> Prims.bool) =
   fun t0 ->
@@ -362,10 +414,28 @@ let rec (context_included :
               FStar_Syntax_Syntax.Binding_univ uu___1) -> true
            | uu___ -> false)
       | uu___ -> false
-let (lookup :
-  FStar_TypeChecker_Env.env ->
-    FStar_Syntax_Syntax.term -> FStar_Syntax_Syntax.typ result)
+let (curry_application :
+  FStar_Syntax_Syntax.term' FStar_Syntax_Syntax.syntax ->
+    (FStar_Syntax_Syntax.term' FStar_Syntax_Syntax.syntax *
+      FStar_Syntax_Syntax.arg_qualifier FStar_Pervasives_Native.option) ->
+      (FStar_Syntax_Syntax.term' FStar_Syntax_Syntax.syntax *
+        FStar_Syntax_Syntax.arg_qualifier FStar_Pervasives_Native.option)
+        Prims.list ->
+        FStar_Compiler_Range.range ->
+          FStar_Syntax_Syntax.term' FStar_Syntax_Syntax.syntax)
   =
+  fun hd ->
+    fun arg ->
+      fun args ->
+        fun p ->
+          let head =
+            FStar_Syntax_Syntax.mk (FStar_Syntax_Syntax.Tm_app (hd, [arg])) p in
+          let t =
+            FStar_Syntax_Syntax.mk (FStar_Syntax_Syntax.Tm_app (head, args))
+              p in
+          t
+let (lookup :
+  env -> FStar_Syntax_Syntax.term -> FStar_Syntax_Syntax.typ result) =
   fun g ->
     fun e ->
       let uu___ = FStar_Hash.lookup (e, FStar_Syntax_Hash.hash_term) table in
@@ -373,12 +443,13 @@ let (lookup :
       | FStar_Pervasives_Native.None -> fail "not in cache"
       | FStar_Pervasives_Native.Some he ->
           let uu___1 =
-            context_included he.he_gamma g.FStar_TypeChecker_Env.gamma in
+            context_included he.he_gamma
+              (g.tcenv).FStar_TypeChecker_Env.gamma in
           if uu___1
-          then FStar_Pervasives.Inl (he.he_res)
+          then (fun uu___2 -> FStar_Pervasives.Inl (he.he_res))
           else fail "not in cache"
 let rec (check_subtype_whnf :
-  FStar_TypeChecker_Env.env ->
+  env ->
     FStar_Syntax_Syntax.term ->
       FStar_Syntax_Syntax.typ -> FStar_Syntax_Syntax.typ -> unit result)
   =
@@ -465,6 +536,19 @@ let rec (check_subtype_whnf :
               let uu___1 = curry_arrow x0 xs0 c0 in
               let uu___2 = curry_arrow x1 xs1 c1 in
               check_subtype_whnf g e uu___1 uu___2
+          | (FStar_Syntax_Syntax.Tm_app (hd0, (arg0, aq0)::[]),
+             FStar_Syntax_Syntax.Tm_app (hd1, (arg1, aq1)::[])) ->
+              let uu___1 = check_equality_whnf g hd0 hd1 in
+              bind uu___1 (fun uu___2 -> check_equality g arg0 arg1)
+          | (FStar_Syntax_Syntax.Tm_app (hd0, arg0::args0),
+             FStar_Syntax_Syntax.Tm_app (hd1, arg1::args1)) ->
+              let uu___1 =
+                curry_application hd0 arg0 args0 t0.FStar_Syntax_Syntax.pos in
+              let uu___2 =
+                curry_application hd1 arg1 args1 t1.FStar_Syntax_Syntax.pos in
+              check_subtype g e uu___1 uu___2
+          | (FStar_Syntax_Syntax.Tm_type u0, FStar_Syntax_Syntax.Tm_type u1)
+              -> check_equality_whnf g t0 t1
           | uu___1 ->
               let uu___2 =
                 let uu___3 = FStar_Syntax_Util.eq_tm t0 t1 in
@@ -490,7 +574,7 @@ let rec (check_subtype_whnf :
                         "Subtyping failed: %s </: %s" uu___7 uu___8 in
                     fail uu___6))
 and (check_subtype :
-  FStar_TypeChecker_Env.env ->
+  env ->
     FStar_Syntax_Syntax.term ->
       FStar_Syntax_Syntax.typ -> FStar_Syntax_Syntax.typ -> unit result)
   =
@@ -508,17 +592,81 @@ and (check_subtype :
                   FStar_TypeChecker_Env.Weak;
                   FStar_TypeChecker_Env.HNF;
                   FStar_TypeChecker_Env.UnfoldUntil
-                    FStar_Syntax_Syntax.delta_constant] g t0 in
+                    FStar_Syntax_Syntax.delta_constant] g.tcenv t0 in
               let t11 =
                 FStar_TypeChecker_Normalize.normalize_refinement
                   [FStar_TypeChecker_Env.Primops;
                   FStar_TypeChecker_Env.Weak;
                   FStar_TypeChecker_Env.HNF;
                   FStar_TypeChecker_Env.UnfoldUntil
-                    FStar_Syntax_Syntax.delta_constant] g t1 in
+                    FStar_Syntax_Syntax.delta_constant] g.tcenv t1 in
               check_subtype_whnf g e t01 t11
+and (check_equality_whnf :
+  env -> FStar_Syntax_Syntax.typ -> FStar_Syntax_Syntax.typ -> unit result) =
+  fun g ->
+    fun t0 ->
+      fun t1 ->
+        let fail1 uu___ =
+          let uu___1 =
+            let uu___2 = FStar_Syntax_Print.term_to_string t0 in
+            let uu___3 = FStar_Syntax_Print.term_to_string t1 in
+            FStar_Compiler_Util.format2 "not equal terms: %s <> %s" uu___2
+              uu___3 in
+          fail uu___1 in
+        let uu___ =
+          let uu___1 = FStar_Syntax_Util.eq_tm t0 t1 in
+          uu___1 = FStar_Syntax_Util.Equal in
+        if uu___
+        then return ()
+        else
+          if g.allow_universe_instantiation
+          then
+            (match ((t0.FStar_Syntax_Syntax.n), (t1.FStar_Syntax_Syntax.n))
+             with
+             | (FStar_Syntax_Syntax.Tm_uinst (f0, us0),
+                FStar_Syntax_Syntax.Tm_uinst (f1, us1)) ->
+                 let uu___2 =
+                   let uu___3 = FStar_Syntax_Util.eq_tm f0 f1 in
+                   uu___3 = FStar_Syntax_Util.Equal in
+                 if uu___2
+                 then
+                   let uu___3 =
+                     FStar_TypeChecker_Rel.teq_nosmt_force g.tcenv t0 t1 in
+                   (if uu___3 then return () else fail1 ())
+                 else fail1 ()
+             | (FStar_Syntax_Syntax.Tm_type u0, FStar_Syntax_Syntax.Tm_type
+                u1) ->
+                 let uu___2 =
+                   FStar_TypeChecker_Rel.teq_nosmt_force g.tcenv t0 t1 in
+                 if uu___2 then return () else fail1 ()
+             | uu___2 -> fail1 ())
+          else fail1 ()
+and (check_equality :
+  env -> FStar_Syntax_Syntax.typ -> FStar_Syntax_Syntax.typ -> unit result) =
+  fun g ->
+    fun t0 ->
+      fun t1 ->
+        let uu___ = FStar_Syntax_Util.eq_tm t0 t1 in
+        match uu___ with
+        | FStar_Syntax_Util.Equal -> return ()
+        | uu___1 ->
+            let t01 =
+              FStar_TypeChecker_Normalize.normalize_refinement
+                [FStar_TypeChecker_Env.Primops;
+                FStar_TypeChecker_Env.Weak;
+                FStar_TypeChecker_Env.HNF;
+                FStar_TypeChecker_Env.UnfoldUntil
+                  FStar_Syntax_Syntax.delta_constant] g.tcenv t0 in
+            let t11 =
+              FStar_TypeChecker_Normalize.normalize_refinement
+                [FStar_TypeChecker_Env.Primops;
+                FStar_TypeChecker_Env.Weak;
+                FStar_TypeChecker_Env.HNF;
+                FStar_TypeChecker_Env.UnfoldUntil
+                  FStar_Syntax_Syntax.delta_constant] g.tcenv t1 in
+            check_equality_whnf g t01 t11
 and (check_subcomp :
-  FStar_TypeChecker_Env.env ->
+  env ->
     FStar_Syntax_Syntax.term ->
       FStar_Syntax_Syntax.comp -> FStar_Syntax_Syntax.comp -> unit result)
   =
@@ -535,239 +683,266 @@ and (check_subcomp :
             check_subtype g e (FStar_Syntax_Util.comp_result c0)
               (FStar_Syntax_Util.comp_result c1)
           else fail "Subcomp failed"
-and (check :
-  FStar_TypeChecker_Env.env ->
-    FStar_Syntax_Syntax.term ->
-      ((FStar_Syntax_Syntax.typ * FStar_Syntax_Syntax.typ
-         FStar_Pervasives_Native.option),
-        Prims.string) FStar_Pervasives.either)
-  =
+and (memo_check :
+  env -> FStar_Syntax_Syntax.term -> FStar_Syntax_Syntax.typ result) =
   fun g ->
     fun e ->
       let uu___ = lookup g e in
       handle_with uu___
         (fun uu___1 ->
-           let r = check' g e in
-           match r with
-           | FStar_Pervasives.Inl res -> (insert g e res; r)
-           | uu___2 -> r)
-and (check' :
-  FStar_TypeChecker_Env.env ->
-    FStar_Syntax_Syntax.term -> FStar_Syntax_Syntax.typ result)
+           fun ctx ->
+             let r = let uu___2 = check' g e in uu___2 ctx in
+             match r with
+             | FStar_Pervasives.Inl res -> (insert g e res; r)
+             | uu___2 -> r)
+and (check :
+  Prims.string ->
+    env -> FStar_Syntax_Syntax.term -> FStar_Syntax_Syntax.typ result)
   =
+  fun msg ->
+    fun g ->
+      fun e ->
+        with_context msg (FStar_Pervasives_Native.Some e)
+          (fun uu___ -> memo_check g e)
+and (check' :
+  env -> FStar_Syntax_Syntax.term -> FStar_Syntax_Syntax.typ result) =
   fun g ->
     fun e ->
-      let uu___ =
-        let uu___1 = FStar_Syntax_Subst.compress e in
-        uu___1.FStar_Syntax_Syntax.n in
-      match uu___ with
-      | FStar_Syntax_Syntax.Tm_meta (t, uu___1) -> check g t
+      let e1 = FStar_Syntax_Subst.compress e in
+      match e1.FStar_Syntax_Syntax.n with
+      | FStar_Syntax_Syntax.Tm_meta (t, uu___) -> memo_check g t
       | FStar_Syntax_Syntax.Tm_uvar (uv, s) ->
-          let uu___1 =
-            let uu___2 = FStar_Syntax_Util.ctx_uvar_typ uv in
-            FStar_Syntax_Subst.subst' s uu___2 in
-          return uu___1
+          let uu___ =
+            let uu___1 = FStar_Syntax_Util.ctx_uvar_typ uv in
+            FStar_Syntax_Subst.subst' s uu___1 in
+          return uu___
       | FStar_Syntax_Syntax.Tm_name x ->
-          let uu___1 = FStar_TypeChecker_Env.lookup_bv g x in
-          (match uu___1 with | (t, uu___2) -> return t)
+          let uu___ = FStar_TypeChecker_Env.lookup_bv g.tcenv x in
+          (match uu___ with | (t, uu___1) -> return t)
       | FStar_Syntax_Syntax.Tm_fvar f ->
-          let uu___1 =
-            FStar_TypeChecker_Env.try_lookup_lid g
+          let uu___ =
+            FStar_TypeChecker_Env.try_lookup_lid g.tcenv
               (f.FStar_Syntax_Syntax.fv_name).FStar_Syntax_Syntax.v in
-          (match uu___1 with
-           | FStar_Pervasives_Native.Some (([], t), uu___2) -> return t
-           | uu___2 -> fail "Missing universes instantiation")
+          (match uu___ with
+           | FStar_Pervasives_Native.Some (([], t), uu___1) -> return t
+           | uu___1 -> fail "Missing universes instantiation")
       | FStar_Syntax_Syntax.Tm_uinst
           ({ FStar_Syntax_Syntax.n = FStar_Syntax_Syntax.Tm_fvar f;
-             FStar_Syntax_Syntax.pos = uu___1;
-             FStar_Syntax_Syntax.vars = uu___2;
-             FStar_Syntax_Syntax.hash_code = uu___3;_},
+             FStar_Syntax_Syntax.pos = uu___;
+             FStar_Syntax_Syntax.vars = uu___1;
+             FStar_Syntax_Syntax.hash_code = uu___2;_},
            us)
           ->
-          let uu___4 =
-            FStar_TypeChecker_Env.try_lookup_and_inst_lid g us
+          let uu___3 =
+            FStar_TypeChecker_Env.try_lookup_and_inst_lid g.tcenv us
               (f.FStar_Syntax_Syntax.fv_name).FStar_Syntax_Syntax.v in
-          (match uu___4 with
+          (match uu___3 with
            | FStar_Pervasives_Native.None -> fail "Top-level name not found"
-           | FStar_Pervasives_Native.Some (t, uu___5) -> return t)
+           | FStar_Pervasives_Native.Some (t, uu___4) -> return t)
       | FStar_Syntax_Syntax.Tm_constant c ->
-          let t =
-            FStar_TypeChecker_TcTerm.tc_constant g e.FStar_Syntax_Syntax.pos
-              c in
-          return t
+          (match c with
+           | FStar_Const.Const_range_of -> fail "Unhandled constant"
+           | FStar_Const.Const_set_range_of -> fail "Unhandled constant"
+           | FStar_Const.Const_reify -> fail "Unhandled constant"
+           | FStar_Const.Const_reflect uu___ -> fail "Unhandled constant"
+           | uu___ ->
+               let t =
+                 FStar_TypeChecker_TcTerm.tc_constant g.tcenv
+                   e1.FStar_Syntax_Syntax.pos c in
+               return t)
       | FStar_Syntax_Syntax.Tm_type u ->
-          let uu___1 = mk_type (FStar_Syntax_Syntax.U_succ u) in
-          return uu___1
+          let uu___ = mk_type (FStar_Syntax_Syntax.U_succ u) in return uu___
       | FStar_Syntax_Syntax.Tm_refine (x, phi) ->
-          let uu___1 =
-            let uu___2 =
-              let uu___3 = FStar_Syntax_Syntax.mk_binder x in [uu___3] in
-            FStar_Syntax_Subst.open_term uu___2 phi in
-          (match uu___1 with
+          let uu___ =
+            let uu___1 =
+              let uu___2 = FStar_Syntax_Syntax.mk_binder x in [uu___2] in
+            FStar_Syntax_Subst.open_term uu___1 phi in
+          (match uu___ with
            | (x1::[], phi1) ->
-               let uu___2 =
-                 check g
+               let uu___1 =
+                 check "refinement head" g
                    (x1.FStar_Syntax_Syntax.binder_bv).FStar_Syntax_Syntax.sort in
-               bind uu___2
+               bind uu___1
                  (fun t ->
-                    let uu___3 = is_type g t in
-                    bind uu___3
+                    let uu___2 = is_type g t in
+                    bind uu___2
                       (fun u ->
-                         let uu___4 =
-                           let g' = FStar_TypeChecker_Env.push_binders g [x1] in
-                           let uu___5 = check g' phi1 in
-                           bind uu___5
+                         let uu___3 =
+                           let g' = push_binders g [x1] in
+                           let uu___4 = check "refinement formula" g' phi1 in
+                           bind uu___4
                              (fun t' ->
-                                let uu___6 = is_type g' t' in
-                                bind uu___6 (fun uu___7 -> return t)) in
-                         with_binders [x1] [u] uu___4)))
-      | FStar_Syntax_Syntax.Tm_abs (xs, body, uu___1) ->
-          let uu___2 = FStar_Syntax_Subst.open_term xs body in
-          (match uu___2 with
-           | (xs1, body1) ->
-               let uu___3 = check_binders g xs1 in
-               bind uu___3
-                 (fun xs_g ->
-                    let uu___4 = xs_g in
-                    match uu___4 with
-                    | (xs2, us, g1) ->
-                        let uu___5 =
-                          let uu___6 = check g1 body1 in
-                          bind uu___6
-                            (fun t ->
-                               let uu___7 =
-                                 let uu___8 = FStar_Syntax_Syntax.mk_Total t in
-                                 FStar_Syntax_Util.arrow xs2 uu___8 in
-                               return uu___7) in
-                        with_binders xs2 us uu___5))
-      | FStar_Syntax_Syntax.Tm_arrow (xs, c) ->
-          let uu___1 = FStar_Syntax_Subst.open_comp xs c in
+                                let uu___5 = is_type g' t' in
+                                bind uu___5 (fun uu___6 -> return t)) in
+                         with_binders [x1] [u] uu___3)))
+      | FStar_Syntax_Syntax.Tm_abs (xs, body, uu___) ->
+          let uu___1 = FStar_Syntax_Subst.open_term xs body in
           (match uu___1 with
-           | (xs1, c1) ->
-               let uu___2 = check_binders g xs1 in
+           | (xs1, body1) ->
+               let uu___2 =
+                 with_context "abs binders" FStar_Pervasives_Native.None
+                   (fun uu___3 -> check_binders g xs1) in
                bind uu___2
                  (fun xs_g ->
                     let uu___3 = xs_g in
                     match uu___3 with
                     | (xs2, us, g1) ->
                         let uu___4 =
-                          let uu___5 = check_comp g1 c1 in
+                          let uu___5 = check "abs body" g1 body1 in
                           bind uu___5
-                            (fun u ->
+                            (fun t ->
                                let uu___6 =
-                                 mk_type
-                                   (FStar_Syntax_Syntax.U_max (u :: us)) in
+                                 let uu___7 = FStar_Syntax_Syntax.mk_Total t in
+                                 FStar_Syntax_Util.arrow xs2 uu___7 in
                                return uu___6) in
                         with_binders xs2 us uu___4))
+      | FStar_Syntax_Syntax.Tm_arrow (xs, c) ->
+          let uu___ = FStar_Syntax_Subst.open_comp xs c in
+          (match uu___ with
+           | (xs1, c1) ->
+               let uu___1 =
+                 with_context "arrow binders" FStar_Pervasives_Native.None
+                   (fun uu___2 -> check_binders g xs1) in
+               bind uu___1
+                 (fun xs_g ->
+                    let uu___2 = xs_g in
+                    match uu___2 with
+                    | (xs2, us, g1) ->
+                        let uu___3 =
+                          let uu___4 =
+                            with_context "arrow comp"
+                              FStar_Pervasives_Native.None
+                              (fun uu___5 -> check_comp g1 c1) in
+                          bind uu___4
+                            (fun u ->
+                               let uu___5 =
+                                 mk_type
+                                   (FStar_Syntax_Syntax.U_max (u :: us)) in
+                               return uu___5) in
+                        with_binders xs2 us uu___3))
       | FStar_Syntax_Syntax.Tm_app (hd, (arg, arg_qual)::[]) ->
-          let uu___1 = check g hd in
-          bind uu___1
+          let uu___ = check "app head" g hd in
+          bind uu___
             (fun t ->
-               let uu___2 = is_tot_arrow g t in
-               bind uu___2
+               let uu___1 = is_tot_arrow g t in
+               bind uu___1
                  (fun x_r ->
-                    let uu___3 = x_r in
-                    match uu___3 with
+                    let uu___2 = x_r in
+                    match uu___2 with
                     | (x, t') ->
-                        let uu___4 = check g arg in
-                        bind uu___4
+                        let uu___3 = check "app arg" g arg in
+                        bind uu___3
                           (fun t_arg ->
-                             let uu___5 =
-                               check_subtype g arg t_arg
-                                 (x.FStar_Syntax_Syntax.binder_bv).FStar_Syntax_Syntax.sort in
-                             bind uu___5
-                               (fun uu___6 ->
-                                  let uu___7 =
-                                    check_arg_qual arg_qual
-                                      x.FStar_Syntax_Syntax.binder_qual in
-                                  bind uu___7
-                                    (fun uu___8 ->
-                                       let uu___9 =
+                             let uu___4 =
+                               with_context "app subtyping"
+                                 FStar_Pervasives_Native.None
+                                 (fun uu___5 ->
+                                    check_subtype g arg t_arg
+                                      (x.FStar_Syntax_Syntax.binder_bv).FStar_Syntax_Syntax.sort) in
+                             bind uu___4
+                               (fun uu___5 ->
+                                  let uu___6 =
+                                    with_context "app arg qual"
+                                      FStar_Pervasives_Native.None
+                                      (fun uu___7 ->
+                                         check_arg_qual arg_qual
+                                           x.FStar_Syntax_Syntax.binder_qual) in
+                                  bind uu___6
+                                    (fun uu___7 ->
+                                       let uu___8 =
                                          FStar_Syntax_Subst.subst
                                            [FStar_Syntax_Syntax.NT
                                               ((x.FStar_Syntax_Syntax.binder_bv),
                                                 arg)] t' in
-                                       return uu___9)))))
+                                       return uu___8)))))
       | FStar_Syntax_Syntax.Tm_app (hd, arg::args) ->
           let head =
             FStar_Syntax_Syntax.mk (FStar_Syntax_Syntax.Tm_app (hd, [arg]))
-              e.FStar_Syntax_Syntax.pos in
+              e1.FStar_Syntax_Syntax.pos in
           let t =
             FStar_Syntax_Syntax.mk (FStar_Syntax_Syntax.Tm_app (head, args))
-              e.FStar_Syntax_Syntax.pos in
-          check g t
+              e1.FStar_Syntax_Syntax.pos in
+          memo_check g t
       | FStar_Syntax_Syntax.Tm_ascribed
-          (e1, (FStar_Pervasives.Inl t, uu___1, eq), uu___2) ->
-          let uu___3 = check g e1 in
-          bind uu___3
+          (e2, (FStar_Pervasives.Inl t, uu___, eq), uu___1) ->
+          let uu___2 = check "ascription head" g e2 in
+          bind uu___2
             (fun te ->
-               let uu___4 = check g t in
-               bind uu___4
+               let uu___3 = check "ascription type" g t in
+               bind uu___3
                  (fun t' ->
-                    let uu___5 = is_type g t' in
-                    bind uu___5
-                      (fun uu___6 ->
-                         let uu___7 = check_subtype g e1 te t in
-                         bind uu___7 (fun uu___8 -> return t))))
+                    let uu___4 = is_type g t' in
+                    bind uu___4
+                      (fun uu___5 ->
+                         let uu___6 =
+                           with_context "ascription subtyping"
+                             FStar_Pervasives_Native.None
+                             (fun uu___7 -> check_subtype g e2 te t) in
+                         bind uu___6 (fun uu___7 -> return t))))
+      | FStar_Syntax_Syntax.Tm_ascribed
+          (uu___, (FStar_Pervasives.Inr e2, uu___1, uu___2), uu___3) ->
+          fail "Effect ascriptions are not handled yet"
       | FStar_Syntax_Syntax.Tm_let ((false, lb::[]), body) ->
-          let uu___1 = lb.FStar_Syntax_Syntax.lbname in
-          (match uu___1 with
+          let uu___ = lb.FStar_Syntax_Syntax.lbname in
+          (match uu___ with
            | FStar_Pervasives.Inl x ->
-               let uu___2 =
-                 let uu___3 =
-                   let uu___4 = FStar_Syntax_Syntax.mk_binder x in [uu___4] in
-                 FStar_Syntax_Subst.open_term uu___3 body in
-               (match uu___2 with
+               let uu___1 =
+                 let uu___2 =
+                   let uu___3 = FStar_Syntax_Syntax.mk_binder x in [uu___3] in
+                 FStar_Syntax_Subst.open_term uu___2 body in
+               (match uu___1 with
                 | (x1::[], body1) ->
-                    let uu___3 =
+                    let uu___2 =
                       FStar_Ident.lid_equals lb.FStar_Syntax_Syntax.lbeff
                         FStar_Parser_Const.effect_Tot_lid in
-                    if uu___3
+                    if uu___2
                     then
-                      let uu___4 = check g lb.FStar_Syntax_Syntax.lbdef in
-                      bind uu___4
+                      let uu___3 =
+                        check "let definition" g lb.FStar_Syntax_Syntax.lbdef in
+                      bind uu___3
                         (fun tdef ->
-                           let uu___5 = check g lb.FStar_Syntax_Syntax.lbtyp in
-                           bind uu___5
+                           let uu___4 =
+                             check "let type" g lb.FStar_Syntax_Syntax.lbtyp in
+                           bind uu___4
                              (fun ttyp ->
-                                let uu___6 = is_type g ttyp in
-                                bind uu___6
+                                let uu___5 = is_type g ttyp in
+                                bind uu___5
                                   (fun u ->
-                                     let uu___7 =
-                                       check_subtype g
-                                         lb.FStar_Syntax_Syntax.lbdef tdef
-                                         ttyp in
-                                     bind uu___7
-                                       (fun uu___8 ->
-                                          let uu___9 =
-                                            let g1 =
-                                              FStar_TypeChecker_Env.push_binders
-                                                g [x1] in
-                                            check g1 body1 in
+                                     let uu___6 =
+                                       with_context "let subtyping"
+                                         FStar_Pervasives_Native.None
+                                         (fun uu___7 ->
+                                            check_subtype g
+                                              lb.FStar_Syntax_Syntax.lbdef
+                                              tdef ttyp) in
+                                     bind uu___6
+                                       (fun uu___7 ->
+                                          let uu___8 =
+                                            let g1 = push_binders g [x1] in
+                                            check "let body" g1 body1 in
                                           with_definition x1 u
                                             lb.FStar_Syntax_Syntax.lbdef
-                                            uu___9))))
+                                            uu___8))))
                     else fail "Let binding is effectful"))
       | FStar_Syntax_Syntax.Tm_match
           (sc, FStar_Pervasives_Native.None, branches,
            FStar_Pervasives_Native.Some
-           { FStar_Syntax_Syntax.residual_effect = uu___1;
+           { FStar_Syntax_Syntax.residual_effect = uu___;
              FStar_Syntax_Syntax.residual_typ = FStar_Pervasives_Native.Some
                t;
-             FStar_Syntax_Syntax.residual_flags = uu___2;_})
+             FStar_Syntax_Syntax.residual_flags = uu___1;_})
           -> fail "Match is not handled yet"
-      | FStar_Syntax_Syntax.Tm_match uu___1 ->
-          fail "Match is not handled yet"
-      | uu___1 ->
-          let uu___2 =
-            let uu___3 = FStar_Syntax_Print.tag_of_term e in
-            FStar_Compiler_Util.format1 "Unexpected term: %s" uu___3 in
-          fail uu___2
+      | FStar_Syntax_Syntax.Tm_match uu___ -> fail "Match is not handled yet"
+      | uu___ ->
+          let uu___1 =
+            let uu___2 = FStar_Syntax_Print.tag_of_term e1 in
+            FStar_Compiler_Util.format1 "Unexpected term: %s" uu___2 in
+          fail uu___1
 and (check_binders :
-  FStar_TypeChecker_Env.env ->
+  env ->
     FStar_Syntax_Syntax.binders ->
       (FStar_Syntax_Syntax.binders * FStar_Syntax_Syntax.universe Prims.list
-        * FStar_TypeChecker_Env.env) result)
+        * env) result)
   =
   fun g ->
     fun xs ->
@@ -775,7 +950,7 @@ and (check_binders :
       | [] -> return ([], [], g)
       | x::xs1 ->
           let uu___ =
-            check g
+            check "binder sort" g
               (x.FStar_Syntax_Syntax.binder_bv).FStar_Syntax_Syntax.sort in
           bind uu___
             (fun t ->
@@ -783,7 +958,7 @@ and (check_binders :
                bind uu___1
                  (fun u ->
                     let uu___2 =
-                      let g' = FStar_TypeChecker_Env.push_binders g [x] in
+                      let g' = push_binders g [x] in
                       let uu___3 = check_binders g' xs1 in
                       bind uu___3
                         (fun xs_g ->
@@ -793,20 +968,68 @@ and (check_binders :
                                return ((x :: xs2), (u :: us), g1)) in
                     with_binders [x] [u] uu___2))
 and (check_comp :
-  FStar_TypeChecker_Env.env ->
-    FStar_Syntax_Syntax.comp -> FStar_Syntax_Syntax.universe result)
-  =
+  env -> FStar_Syntax_Syntax.comp -> FStar_Syntax_Syntax.universe result) =
   fun g ->
     fun c ->
       let uu___ = FStar_Syntax_Util.is_tot_or_gtot_comp c in
       if uu___
       then
-        let uu___1 = check g (FStar_Syntax_Util.comp_result c) in
+        let uu___1 = check "comp result" g (FStar_Syntax_Util.comp_result c) in
         bind uu___1 (fun t -> is_type g t)
       else fail "Computation type is not Tot or GTot"
 and (universe_of :
+  env -> FStar_Syntax_Syntax.typ -> FStar_Syntax_Syntax.universe result) =
+  fun g ->
+    fun t ->
+      let uu___ = check "universe of" g t in
+      bind uu___ (fun t1 -> is_type g t1)
+let (check_term_top :
   FStar_TypeChecker_Env.env ->
-    FStar_Syntax_Syntax.typ -> FStar_Syntax_Syntax.universe result)
+    FStar_Syntax_Syntax.term -> FStar_Syntax_Syntax.typ -> unit result)
   =
   fun g ->
-    fun t -> let uu___ = check g t in bind uu___ (fun t1 -> is_type g t1)
+    fun e ->
+      fun t ->
+        let g1 = { tcenv = g; allow_universe_instantiation = false } in
+        let uu___ = check "top" g1 e in
+        bind uu___
+          (fun te ->
+             with_context "top-level subtyping" FStar_Pervasives_Native.None
+               (fun uu___1 ->
+                  check_subtype
+                    { tcenv = (g1.tcenv); allow_universe_instantiation = true
+                    } e te t))
+let (check_term :
+  FStar_TypeChecker_Env.env ->
+    FStar_Syntax_Syntax.term ->
+      FStar_Syntax_Syntax.typ ->
+        (FStar_Syntax_Syntax.typ FStar_Pervasives_Native.option, error)
+          FStar_Pervasives.either)
+  =
+  fun g ->
+    fun e ->
+      fun t ->
+        let uu___ = let uu___1 = check_term_top g e t in uu___1 [] in
+        match uu___ with
+        | FStar_Pervasives.Inl (uu___1, g1) -> FStar_Pervasives.Inl g1
+        | FStar_Pervasives.Inr err -> FStar_Pervasives.Inr err
+let (print_error : error -> Prims.string) =
+  fun err ->
+    let rec print_context depth ctx =
+      match ctx with
+      | [] -> ""
+      | (msg, topt)::tl ->
+          let hd =
+            let uu___ =
+              match topt with
+              | FStar_Pervasives_Native.None -> ""
+              | FStar_Pervasives_Native.Some t ->
+                  FStar_Syntax_Print.term_to_string t in
+            FStar_Compiler_Util.format3 "%s %s (%s)\n" depth msg uu___ in
+          let tl1 = print_context (Prims.op_Hat depth ">") tl in
+          Prims.op_Hat hd tl1 in
+    let uu___ = err in
+    match uu___ with
+    | (ctx, msg) ->
+        let uu___1 = print_context "" (FStar_Compiler_List.rev ctx) in
+        FStar_Compiler_Util.format2 "%s%s" uu___1 msg
