src/typechecker/FStar.TypeChecker.Core.fsti
@@ -6,10 +6,13 @@ module S = FStar.Syntax.Syntax
 module R = FStar.Compiler.Range
 module U = FStar.Syntax.Util
 
-
 val clear_memo_table (_:unit)
   : unit
 
-val check (g:Env.env) (e:term)
-  : either (typ & option typ) string
+val error : Type0
 
+val check_term (g:Env.env) (e:term) (t:typ)
+  : either (option typ) error
+
+val print_error (err:error)
+  : string
